@prefix : <http://purl.org/lis590OD/Fall17/Employment_Ontology#> .
@prefix dc: <http://purl.org/dc/elements/1.1/> .
@prefix tl: <http://purl.org/NET/c4dm/timeline.owl#> .
@prefix dbp: <http://dbpedia.org/resource/> .
@prefix geo: <http://www.w3.org/2003/01/geo/wgs84_pos#> .
@prefix org: <http://www.w3.org/ns/org#> .
@prefix owl: <http://www.w3.org/2002/07/owl#> .
@prefix rdf: <http://www.w3.org/1999/02/22-rdf-syntax-ns#> .
@prefix xml: <http://www.w3.org/XML/1998/namespace> .
@prefix xsd: <http://www.w3.org/2001/XMLSchema#> .
@prefix xsp: <http://www.owl-ontologies.com/2005/08/07/xsp.owl#> .
@prefix foaf: <http://xmlns.com/foaf/0.1/> .
@prefix prov: <http://www.w3.org/ns/prov#> .
@prefix rdfs: <http://www.w3.org/2000/01/rdf-schema#> .
@prefix skos: <http://www.w3.org/2004/02/skos/core#> .
@prefix swrl: <http://www.w3.org/2003/11/swrl#> .
@prefix wped: <http://en.wikipedia.org/wiki/> .
@prefix dolce: <http://ontology.ip.rm.cnr.it/ontologies/DOLCE-Lite#> .
@prefix event: <http://purl.org/NET/c4dm/event.owl#> .
@prefix swrlb: <http://www.w3.org/2003/11/swrlb#> .
@prefix dcterms: <http://purl.org/dc/terms/> .
@prefix protege: <http://protege.stanford.edu/plugins/owl/protege#> .
@base <http://purl.org/lis590OD/Fall17/Employment_Ontology#> .

<http://purl.org/lis590OD/Fall17/Employment_Ontology> rdf:type owl:Ontology ;
                                  owl:imports <http://purl.org/lis590od/Fall17/OrgRel> .

#################################################################
#    Object Properties
#################################################################

###  http://purl.org/NET/c4dm/event.owl#place
event:place rdfs:domain :EmploymentEvent ,
                        :SelfEmployed .


###  http://www.example.com/Example#Position
:Position rdf:type owl:ObjectProperty ;
          rdfs:domain :EmploymentEvent ;
          rdfs:range [ rdf:type owl:Restriction ;
                       owl:onProperty owl:topDataProperty ;
                       owl:allValuesFrom xsd:string
                     ] ;
          rdfs:comment "The title or position an individual holds at a company in an employment event" ;
          rdfs:label "position" .


###  http://www.example.com/Example#employmentType
:employmentType rdf:type owl:ObjectProperty ;
                rdfs:domain :EmploymentEvent .


###  http://www.example.com/Example#full-time
:full-time rdf:type owl:ObjectProperty ;
           rdfs:subPropertyOf :employmentType ;
           rdfs:domain :EmploymentEvent ;
           owl:propertyDisjointWith :part-time .


###  http://www.example.com/Example#part-time
:part-time rdf:type owl:ObjectProperty ;
           rdfs:subPropertyOf :employmentType ;
           rdfs:domain :EmploymentEvent ;
           rdfs:comment "A type of employment, where an individual works fewer hours than full-time." ;
           rdfs:label "part-time" .


#################################################################
#    Data properties
#################################################################

###  http://www.example.com/Example#weeklyHours
:weeklyHours rdf:type owl:DatatypeProperty ;
             rdfs:subPropertyOf <http://www.w3.org/2006/time#hours> ;
             rdfs:domain :EmploymentEvent ,
                         :SelfEmployed ;
             rdfs:range xsd:nonNegativeInteger ;
             rdfs:label "weeklyEmploymentHours" .


#################################################################
#    Classes
#################################################################

###  http://www.example.com/Example#EmployingOrganization
:EmployingOrganization rdf:type owl:Class ;
                       rdfs:subClassOf foaf:Organization ;
                       rdfs:comment "The organization that employs an agent in an Employment Event" ;
                       rdfs:label "Employing Organization" .


###  http://www.example.com/Example#EmploymentEvent
:EmploymentEvent rdf:type owl:Class ;
                 rdfs:subClassOf <http://purl.org/lis590od/Fall17/OrgRel#OrganizationRelationship> ;
                 rdfs:comment "Instance of employment, where an individual is employed by a organization" ;
                 rdfs:label "Employment Event" .


###  http://www.example.com/Example#SelfEmployed
:SelfEmployed rdf:type owl:Class ;
              rdfs:subClassOf :WorkRelationship ;
              rdfs:comment "Instance of employment where the individual is not employed by a company, and is their own boss" ;
              rdfs:label "Self Employed" .


###  http://www.example.com/Example#Unemployed
:Unemployed rdf:type owl:Class ;
            rdfs:subClassOf :WorkRelationship ;
            rdfs:comment "Event where a person is not employed by either a company or self" ;
            rdfs:label "Unemployed" .


###  http://www.example.com/Example#WorkRelationship
:WorkRelationship rdf:type owl:Class ;
                  rdfs:subClassOf <http://purl.org/lis590od/Fall17/OrgRel#OrganizationRelationship> .


###  Generated by the OWL API (version 4.2.8.20170104-2310) https://github.com/owlcs/owlapi
