@prefix : <http://purl.org/lis590OD/Fall17/Employment_Ontology#> .
@prefix dc: <http://purl.org/dc/elements/1.1/> .
@prefix tl: <http://purl.org/NET/c4dm/timeline.owl#> .
@prefix dbp: <http://dbpedia.org/resource/> .
@prefix geo: <http://www.w3.org/2003/01/geo/wgs84_pos#> .
@prefix org: <http://www.w3.org/ns/org#> .
@prefix owl: <http://www.w3.org/2002/07/owl#> .
@prefix rdf: <http://www.w3.org/1999/02/22-rdf-syntax-ns#> .
@prefix xml: <http://www.w3.org/XML/1998/namespace> .
@prefix xsd: <http://www.w3.org/2001/XMLSchema#> .
@prefix xsp: <http://www.owl-ontologies.com/2005/08/07/xsp.owl#> .
@prefix foaf: <http://xmlns.com/foaf/0.1/> .
@prefix prov: <http://www.w3.org/ns/prov#> .
@prefix rdfs: <http://www.w3.org/2000/01/rdf-schema#> .
@prefix skos: <http://www.w3.org/2004/02/skos/core#> .
@prefix swrl: <http://www.w3.org/2003/11/swrl#> .
@prefix wped: <http://en.wikipedia.org/wiki/> .
@prefix dolce: <http://ontology.ip.rm.cnr.it/ontologies/DOLCE-Lite#> .
@prefix event: <http://purl.org/NET/c4dm/event.owl#> .
@prefix swrlb: <http://www.w3.org/2003/11/swrlb#> .
@prefix dcterms: <http://purl.org/dc/terms/> .
@prefix protege: <http://protege.stanford.edu/plugins/owl/protege#> .
@base <http://purl.org/lis590OD/Fall17/Employment_Ontology> .

<http://purl.org/lis590OD/Fall17/Employment_Ontology> rdf:type owl:Ontology ;
                                                       owl:imports <http://purl.org/lis590od/Fall17/OrgRel> .

#################################################################
#    Object Properties
#################################################################

###  http://purl.org/lis590OD/Fall17/Employment_Ontology#EmploymentLocation
:EmploymentLocation rdf:type owl:ObjectProperty ;
                    rdfs:subPropertyOf event:place ;
                    rdfs:domain :EmploymentEvent ,
                                :WorkRelationship ;
                    rdfs:range [ rdf:type owl:Restriction ;
                                 owl:onProperty event:place ;
                                 owl:someValuesFrom geo:SpatialThing
                               ] ;
                    rdfs:comment "A location where a person is employed udring an employment event. Multiple locations may be involved in an employment event, such as different branch locations of a company"@en ;
                    rdfs:label "EmploymentLocation"@en .


###  http://purl.org/lis590OD/Fall17/Employment_Ontology#Position
:Position rdf:type owl:ObjectProperty ;
          rdfs:domain :Employee ;
          rdfs:range [ rdf:type owl:Restriction ;
                       owl:onProperty owl:topDataProperty ;
                       owl:allValuesFrom xsd:string
                     ] ;
          rdfs:comment "The title or position an individual holds at a company in an employment event" ;
          rdfs:label "position"@en .


###  http://purl.org/lis590OD/Fall17/Employment_Ontology#studentPosition
:studentPosition rdf:type owl:ObjectProperty ;
                 rdfs:subPropertyOf :Position ;
                 rdfs:domain :Student ;
                 rdfs:range :GraduateStudent ,
                            :HighSchoolStudent ,
                            :MiddleSchoolStudent ,
                            :UndergradStudent ;
                 rdfs:comment "The position a student holds in relation to an employment event or work relationship"@en ;
                 rdfs:label "studentPosition"@en .


#################################################################
#    Data properties
#################################################################

###  http://purl.org/lis590OD/Fall17/Employment_Ontology#employmentEndDate
:employmentEndDate rdf:type owl:DatatypeProperty ;
                   rdfs:domain :EmploymentEvent ,
                               :WorkRelationship ;
                   rdfs:range xsd:gYearMonth ;
                   rdfs:comment "Date when an employment or work event (year, month) ends. Each employment event may only have 0 or 1 employment end date"@en ;
                   rdfs:label "employmentEventEndDate"@en .


###  http://purl.org/lis590OD/Fall17/Employment_Ontology#employmentStartDate
:employmentStartDate rdf:type owl:DatatypeProperty ;
                     rdfs:domain :EmploymentEvent ,
                                 :WorkRelationship ;
                     rdfs:range xsd:gYearMonth ;
                     rdfs:comment "Date (year, month) when an employment event or work relationship started"@en ;
                     rdfs:label "employmentEventStartDate"@en .

[ rdf:type owl:Axiom ;
   owl:annotatedSource :employmentStartDate ;
   owl:annotatedProperty rdfs:range ;
   owl:annotatedTarget xsd:gYearMonth ;
   rdfs:comment ""
 ] .


###  http://purl.org/lis590OD/Fall17/Employment_Ontology#emplymentType
:emplymentType rdf:type owl:DatatypeProperty ;
               rdfs:domain :EmploymentEvent ,
                           :WorkRelationship ;
               rdfs:range [ rdf:type rdfs:Datatype ;
                            owl:oneOf [ rdf:type rdf:List ;
                                        rdf:first "full-time" ;
                                        rdf:rest [ rdf:type rdf:List ;
                                                   rdf:first "part-time" ;
                                                   rdf:rest rdf:nil
                                                 ]
                                      ]
                          ] ;
               rdfs:comment "Type of employment, either as part-time or full-time" ;
               rdfs:label "employmentType"@en .


###  http://purl.org/lis590OD/Fall17/Employment_Ontology#full-time
:full-time rdf:type owl:DatatypeProperty ;
           rdfs:subPropertyOf :emplymentType ;
           owl:propertyDisjointWith :part-time ;
           rdfs:comment "An employment type where an individual works more hours than full-time. Number of hours iss not defined to allow wider use of this property."@en ;
           rdfs:label "full-time"@en .


###  http://purl.org/lis590OD/Fall17/Employment_Ontology#part-time
:part-time rdf:type owl:DatatypeProperty ;
           rdfs:subPropertyOf :emplymentType ;
           rdfs:comment "A type of employment, where the individual works less than full time. Number of hours is not defined to allow wider use of this property"@en ;
           rdfs:label "part-time"@en .


###  http://purl.org/lis590OD/Fall17/Employment_Ontology#weeklyHours
:weeklyHours rdf:type owl:DatatypeProperty ;
             rdfs:subPropertyOf <http://www.w3.org/2006/time#hours> ;
             rdfs:domain :EmploymentEvent ,
                         :SelfEmployed ;
             rdfs:range xsd:nonNegativeInteger ;
             rdfs:comment "The amount of hours a person works in a week, in an employment event" ;
             rdfs:label "weeklyEmploymentHours"@en .


#################################################################
#    Classes
#################################################################

###  http://purl.org/lis590OD/Fall17/Employment_Ontology#Employee
:Employee rdf:type owl:Class ;
          rdfs:subClassOf foaf:Person ;
          rdfs:comment "A person who is employed. The individual can be self employed, or employed by an organization." ;
          rdfs:label "Employee"@en .


###  http://purl.org/lis590OD/Fall17/Employment_Ontology#EmployingOrganization
:EmployingOrganization rdf:type owl:Class ;
                       rdfs:subClassOf foaf:Organization ;
                       rdfs:comment "The organization that employs an agent in an Employment Event" ;
                       rdfs:label "Employing Organization"@en .


###  http://purl.org/lis590OD/Fall17/Employment_Ontology#EmploymentEvent
:EmploymentEvent rdf:type owl:Class ;
                 rdfs:subClassOf <http://purl.org/lis590od/Fall17/OrgRel#OrganizationRelationship> ;
                 rdfs:comment "Instance of employment, where an individual is employed by a organization" ;
                 rdfs:label "Employment Event"@en .


###  http://purl.org/lis590OD/Fall17/Employment_Ontology#GraduateStudent
:GraduateStudent rdf:type owl:Class ;
                 rdfs:subClassOf :Student ;
                 rdfs:comment "Student is enrolled in Graduate program, includes Masters, PhD"@en ;
                 rdfs:label "GraduateStudent"@en .


###  http://purl.org/lis590OD/Fall17/Employment_Ontology#HighSchoolStudent
:HighSchoolStudent rdf:type owl:Class ;
                   rdfs:subClassOf :Student ;
                   rdfs:comment "Student Attends High School"@en ;
                   rdfs:label "HighSchoolStudent"@en .


###  http://purl.org/lis590OD/Fall17/Employment_Ontology#MiddleSchoolStudent
:MiddleSchoolStudent rdf:type owl:Class ;
                     rdfs:subClassOf :Student ;
                     rdfs:comment "Student attends a Middle School"@en ;
                     rdfs:label "MiddleSchoolStudent"@en .


###  http://purl.org/lis590OD/Fall17/Employment_Ontology#Retired
:Retired rdf:type owl:Class ;
         rdfs:subClassOf :WorkRelationship ;
         rdfs:comment "An individual once held employment but is no longer working"@en ;
         rdfs:label "Retired"@en .


###  http://purl.org/lis590OD/Fall17/Employment_Ontology#SelfEmployed
:SelfEmployed rdf:type owl:Class ;
              rdfs:subClassOf :WorkRelationship ;
              rdfs:comment "Instance of employment where the individual is not employed by a company, and is their own boss" ;
              rdfs:label "Self-employed"@en .


###  http://purl.org/lis590OD/Fall17/Employment_Ontology#Student
:Student rdf:type owl:Class ;
         rdfs:subClassOf foaf:Person ;
         rdfs:comment "An individual who is attending school"@en ;
         rdfs:label "Student"@en .


###  http://purl.org/lis590OD/Fall17/Employment_Ontology#StudentEmploymentEvent
:StudentEmploymentEvent rdf:type owl:Class ;
                        rdfs:subClassOf :EmploymentEvent ;
                        rdfs:comment "An employment event where the individual has student as their position, and the employing organization is the school the indiviual attends. A student may have other concurrent employment events or work relationships"@en ;
                        rdfs:label "StudentEmploymentEvent"@en .


###  http://purl.org/lis590OD/Fall17/Employment_Ontology#Supervisor
:Supervisor rdf:type owl:Class ;
            rdfs:subClassOf :Employee ;
            rdfs:comment "An employee who oversees or supervises other employees" ;
            rdfs:label "Supervisor"@en .


###  http://purl.org/lis590OD/Fall17/Employment_Ontology#UndergradStudent
:UndergradStudent rdf:type owl:Class ;
                  rdfs:subClassOf :Student ;
                  rdfs:comment "Student is enrolled in Associates or Bachelors program"@en ;
                  rdfs:label "UndergraduateStudent"@en .


###  http://purl.org/lis590OD/Fall17/Employment_Ontology#Unemployed
:Unemployed rdf:type owl:Class ;
            rdfs:subClassOf :WorkRelationship ;
            rdfs:comment "Event where a person is not employed by either a company or self" ;
            rdfs:label "Unemployed"@en .


###  http://purl.org/lis590OD/Fall17/Employment_Ontology#WorkRelationship
:WorkRelationship rdf:type owl:Class ;
                  rdfs:subClassOf event:Event ;
                  rdfs:comment "A event relating a person and employment, but doesn't include an organization. Can include unemployment and self employment" ;
                  rdfs:label "WorkRelationship"@en .


###  Generated by the OWL API (version 4.2.8.20170104-2310) https://github.com/owlcs/owlapi
